confirmed that INV: "forall (v,chunk) in gv, v:chunk" is the invariant to prove store;load is identical.
In CompCert, there are similar lemmas. The lemmas are used by spilling
pass, and stack records layout pass where they need to show register
spilling and reloading is identical. In the CompCert Memory Model, we
cannot prove that
  if store ptr v; r = load ptr, then [r] = [v]
For example, when v is 0xffff of type int8, r is 0xff, so, we only have 
  [r] = (t)[v] where ptr:t*
This is not suprising, because memory st/ld pair is an implicit
conversion. 

In CompCert, the spilling pass does not need to prove [r]=[v] because
the target language uses an 'abstract' stack that proves this property
for free. They need to prove this in the stack layout pass. At that
pass, CompCert concretly uses i32 chunks for any supported int (i8, i16,
i32) values n CompCert; and double slots for both float and double
values. Luckily, (t)[v] = [v] when t = i32 or double in CompCert, so,
the property holds. I think this is because C spec does not specify how
many bytes to hold i8 and i16 values on stack. (Note, when t=float, 
double-single precision conversion is needed).

LLVM is byte-oriented, and requires the number of bytes to hold a value
is the minimal bytes to contain the corresponding bitsize up to
rounding. So, we need a more precise low-level t than CompCert---chunk
that relates values' size and types' bitsize, and show that the opsem preserves 
INV.  Then we should have:
  if ptr:chunk_of(t*), v:chunk_of(t), and store ptr v; r = load ptr, 
  then [r] = [v].

NOTE: this does not mean LLVM is sound. Because undef can be of any
chunk.



git-svn-id: https://webdav.seas.upenn.edu/svn/sol/vol@3817 eef5ea85-cc2e-0410-bd84-0fae1f012da8

src3.0/Vellvm/genericvalues.v
@@ -31,6 +31,20 @@ Definition mptr := GenericValue.
 Definition null : GenericValue :=
   (Vptr Mem.nullptr (Int.repr 31 0), Mint 31)::nil.
 
+Definition gv_lessdef (gv1 gv2:GenericValue) : Prop :=
+List.Forall2 (fun vm1 vm2 =>
+              let '(v1, cm1) := vm1 in
+              let '(v2, cm2) := vm2 in
+              Val.lessdef v1 v2 /\ cm1 = cm2) gv1 gv2.
+
+Definition gv_has_chunk (gv:GenericValue): Prop :=
+List.Forall (fun vm => 
+             let '(v, mc) := vm in
+             Val.has_chunk v mc) gv.
+
+Definition gv_lessdef_list (gvs1 gvs2:list GenericValue) : Prop :=
+List.Forall2 gv_lessdef gvs1 gvs2.
+
 Fixpoint eq_gv (gv1 gv2:GenericValue) : bool :=
 match gv1, gv2 with
 | nil, nil => true
@@ -134,6 +148,15 @@ Definition flatten_typs (TD:TargetData) (lt:list_typ)
   : option (list memory_chunk) :=
 let '(los, nts) := TD in
 flatten_typs_aux TD (flatten_typ_for_namedts TD los nts) lt.
+
+Definition gv_has_type (TD:LLVMtd.TargetData) (gv:GenericValue) 
+  (t:LLVMsyntax.typ) : Prop :=
+match flatten_typ TD t with
+| None => False
+| Some ts =>
+    List.Forall2 (fun v mc => Val.has_type v (AST.type_of_chunk mc)) 
+                 (fst (List.split gv)) ts
+end.
 
 Definition mc2undefs (mc:list memory_chunk) : GenericValue :=
 List.fold_right 
@@ -2386,5 +2409,11 @@ Proof.
     ].
 Qed.
 
+Lemma gv_lessdef_ref: forall gv, gv_lessdef gv gv.
+Proof.
+  unfold gv_lessdef.
+  induction gv as [|[]]; auto.
+Qed.
+    
 End LLVMgv.
 
